theories/RTac/BIMap.v
@@ -1,0 +1,603 @@
+(** Bounded Instantiated Maps **)
+Require Import Coq.Bool.Bool.
+Require Import Coq.Classes.Morphisms.
+Require Import Coq.Relations.Relations.
+Require Import ExtLib.Core.RelDec.
+Require Import ExtLib.Structures.Monad.
+Require Import ExtLib.Structures.Traversable.
+Require Import ExtLib.Data.Option.
+Require Import ExtLib.Data.Prop.
+Require Import ExtLib.Data.Pair.
+Require Import ExtLib.Data.List.
+Require Import ExtLib.Data.ListFirstnSkipn.
+Require Import ExtLib.Data.HList.
+Require Import ExtLib.Data.Monads.OptionMonad.
+Require Import ExtLib.Tactics.
+Require Import MirrorCore.ExprI.
+Require Import MirrorCore.SubstI.
+Require Import MirrorCore.VariablesI.
+Require Import MirrorCore.ExprDAs.
+Require Import MirrorCore.Subst.FMapSubst.
+
+Require Import MirrorCore.Util.Quant.
+Require Import MirrorCore.Util.Forwardy.
+
+Set Implicit Arguments.
+Set Strict Implicit.
+
+Section parameterized.
+  Variable typ : Type.
+  Variable expr : Type.
+
+  Context {RType_typ : RType typ}.
+  Context {RTypeOk_typ : RTypeOk}.
+  Context {Typ0_Prop : Typ0 _ Prop}.
+  Context {Expr_expr : Expr RType_typ expr}.
+  Context {ExprOk_expr : ExprOk Expr_expr}.
+  Context {ExprVar_expr : ExprVar expr}.
+  Context {ExprVarOk_expr : ExprVarOk _}.
+  Context {ExprUVar_expr : ExprUVar expr}.
+  Context {ExprUVarOk_expr : ExprUVarOk _}.
+  Context {MentionsAny_expr : MentionsAny expr}.
+  Context {MentionsAnyOk_expr : MentionsAnyOk _ _ _}.
+
+  Local Instance RelDec_eq_typ : RelDec (@eq typ) :=
+    RelDec_Rty _.
+  Local Instance RelDecOk_eq_typ : RelDec_Correct RelDec_eq_typ :=
+    @RelDec_Correct_Rty _ _ _.
+
+  Local Existing Instance SUBST.Subst_subst.
+  Local Existing Instance SUBST.SubstOk_subst.
+  Local Existing Instance SUBST.SubstOpen_subst.
+  Local Existing Instance SUBST.SubstOpenOk_subst.
+
+  Definition amap : Type := SUBST.raw expr.
+  Definition WellFormed_amap : amap -> Prop := @SUBST.WellFormed _ _.
+  Definition amap_empty : amap := UVarMap.MAP.empty _.
+  Definition amap_lookup : nat -> amap -> option expr :=
+    @UVarMap.MAP.find _.
+  Definition amap_check_set : nat -> expr -> amap -> option amap :=
+    @SUBST.raw_set _ _.
+  Definition amap_instantiate (f : nat -> option expr) : amap -> amap :=
+    UVarMap.MAP.map (fun e => instantiate f 0 e).
+  Definition amap_substD
+  : forall (tus tvs : tenv typ), amap -> option (exprT tus tvs Prop) :=
+    @SUBST.raw_substD _ _ _ _.
+  Definition amap_is_full (* min : uvar *) (len : nat) (m : amap) : bool :=
+    UVarMap.MAP.cardinal m ?[ eq ] len.
+  Definition amap_domain (m : amap) : list uvar :=
+    map fst (UVarMap.MAP.elements m).
+
+  Definition Forall_amap (P : uvar -> expr -> Prop) (m : amap) : Prop :=
+    forall u e,
+      amap_lookup u m = Some e ->
+      P u e.
+
+  Lemma Forall_amap_empty
+  : forall P, Forall_amap P amap_empty.
+  Proof.
+    clear. intros.
+    red. unfold amap_lookup, amap_empty.
+    intros. rewrite FMapSubst.SUBST.FACTS.empty_o in H. congruence.
+  Qed.
+
+
+  Definition WellFormed_bimap (min : nat) (len : nat) (m : amap)
+  : Prop :=
+    (** 'acyclic' **)
+    SUBST.WellFormed m /\
+    (** only in this range **)
+    Forall_amap (fun k _ => min <= k < min + len) m /\
+    (** no forward pointers **)
+    Forall_amap (fun k e => forall u'',
+                              mentionsU u'' e = true ->
+                              u'' < min + len) m.
+
+  Lemma WellFormed_bimap_empty
+  : forall a b, WellFormed_bimap a b amap_empty.
+  Proof.
+    clear - Expr_expr. red.
+    intros. refine (conj _ (conj _ _));
+            eauto using SUBST.WellFormed_empty, Forall_amap_empty.
+    eapply SUBST.WellFormed_empty.
+  Qed.
+
+  Lemma WellFormed_bimap_WellFormed_amap
+  : forall a b s,
+      WellFormed_bimap a b s ->
+      WellFormed_amap s.
+  Proof.
+    destruct 1. assumption.
+  Qed.
+
+  Lemma amap_instantiates_substD
+  : forall tus tvs C (_ : CtxLogic.ExprTApplicative C) f s sD a b,
+      WellFormed_bimap a b s ->
+      amap_substD tus tvs s = Some sD ->
+      sem_preserves_if_ho C f ->
+      exists sD',
+        amap_substD tus tvs (amap_instantiate f s) = Some sD' /\
+        C (fun us vs => sD us vs <-> sD' us vs).
+  Proof.
+    unfold amap_instantiate.
+    intros.
+    eapply SUBST.raw_substD_instantiate_ho in H2; eauto.
+    forward_reason.
+    eexists; split; eauto.
+    revert H3.
+    eapply CtxLogic.exprTAp.
+    eapply CtxLogic.exprTPure.
+    intros us vs.
+    clear. tauto.
+  Qed.
+
+  Lemma amap_lookup_substD
+  : forall (s : amap) (uv : uvar) (e : expr),
+      amap_lookup uv s = Some e ->
+      forall (tus tvs : list typ)
+             (sD : hlist typD tus -> hlist typD tvs -> Prop),
+        amap_substD tus tvs s = Some sD ->
+        exists
+          (t : typ) (val : exprT tus tvs (typD t))
+          (get : hlist typD tus -> typD t),
+          nth_error_get_hlist_nth typD tus uv =
+          Some (existT (fun t0 : typ => hlist typD tus -> typD t0) t get) /\
+          exprD' tus tvs e t = Some val /\
+          (forall (us : hlist typD tus) (vs : hlist typD tvs),
+             sD us vs -> get us = val us vs).
+  Proof. eapply SUBST.substD_lookup'. Qed.
+
+  Lemma amap_domain_WellFormed
+  : forall (s : amap) (ls : list uvar),
+       WellFormed_amap s ->
+       amap_domain s = ls ->
+       forall n : nat, In n ls <-> amap_lookup n s <> None.
+  Proof. eapply SUBST.WellFormed_domain. Qed.
+
+  Lemma amap_lookup_normalized
+  : forall (s : amap) (e : expr) (u : nat),
+      WellFormed_amap s ->
+      amap_lookup u s = Some e ->
+      forall (u' : nat) (e' : expr),
+        amap_lookup u' s = Some e' -> mentionsU u' e = false.
+  Proof. eapply SUBST.normalized_fmapsubst. Qed.
+
+  Lemma amap_lookup_amap_instantiate
+  : forall u f m,
+      amap_lookup u (amap_instantiate f m) =
+      match amap_lookup u m with
+        | None => None
+        | Some e => Some (instantiate f 0 e)
+      end.
+  Proof.
+    unfold amap_lookup, amap_instantiate; intros.
+    apply SUBST.FACTS.map_o.
+  Qed.
+
+  Lemma syn_check_set
+  : forall uv e s s',
+      WellFormed_amap s ->
+      amap_check_set uv e s = Some s' ->
+      let e' := instantiate (fun u => amap_lookup u s) 0 e in
+      WellFormed_amap s' /\
+      mentionsU uv e'= false /\
+      forall u,
+        amap_lookup u s' =
+        if uv ?[ eq ] u then Some e'
+        else
+          match amap_lookup u s with
+            | None => None
+            | Some e =>
+              Some (instantiate (fun u =>
+                                   if uv ?[ eq ] u then Some e'
+                                   else None) 0 e)
+          end.
+  Proof.
+    intros. unfold amap_check_set, SUBST.raw_set in *.
+    forward. inv_all; subst.
+    split.
+    { eapply SUBST.raw_set_WellFormed; eauto.
+      instantiate (1 := e). instantiate (1 := uv).
+      unfold amap_check_set, SUBST.raw_set in *.
+      rewrite H0. reflexivity. }
+    split.
+    { assumption. }
+    intros.
+    unfold amap_lookup.
+    rewrite SUBST.FACTS.add_o.
+    destruct (SUBST.PROPS.F.eq_dec uv u); subst.
+    { rewrite rel_dec_eq_true; eauto with typeclass_instances. }
+    { rewrite rel_dec_neq_false; eauto with typeclass_instances.
+      unfold SUBST.raw_instantiate.
+      rewrite SUBST.FACTS.map_o.
+      destruct (UVarMap.MAP.find u s); try reflexivity. }
+  Qed.
+
+  Lemma WellFormed_bimap_check_set
+  : forall uv e s min len s',
+      amap_check_set uv e s = Some s' ->
+      (forall u, mentionsU u e = true -> u < min + len) ->
+      min <= uv < min + len ->
+      WellFormed_bimap min len s ->
+      WellFormed_bimap min len s'.
+  Proof.
+    intros.
+    eapply syn_check_set in H; eauto.
+    red in H2. red.
+    { forward_reason.
+      split; auto.
+      split.
+      { red in H3. red.
+        intros.
+        rewrite H7 in H8.
+        consider (uv ?[ eq ] u); intros; subst.
+        omega.
+        forward. eapply H3; eauto. }
+      { red in H4; red; intros.
+        rewrite H7 in H8; clear H7.
+        consider (uv ?[ eq ] u); intros; subst.
+        { inv_all; subst.
+          eapply mentionsU_instantiate in H9.
+          destruct H9.
+          { eapply H0. tauto. }
+          { forward_reason.
+            eapply H4 in H7. eauto. eauto. } }
+        { forward.
+          inv_all; subst.
+          eapply mentionsU_instantiate in H9.
+          destruct H9.
+          { forward_reason.
+            consider (uv ?[ eq ] u''); intros; subst; try congruence.
+            eauto. }
+          { forward_reason.
+            consider (uv ?[ eq ] x); intros; subst; try congruence.
+            inv_all; subst.
+            eapply mentionsU_instantiate in H11.
+            destruct H11.
+            { forward_reason. eauto. }
+            { forward_reason. eauto. } } } } }
+    { destruct H2. assumption. }
+  Qed.
+
+  Lemma Forall_amap_instaniate
+  : forall (P Q : uvar -> expr -> Prop) f m,
+      (forall u e, Q u e -> P u (instantiate f 0 e)) ->
+      Forall_amap Q m ->
+      Forall_amap P (amap_instantiate f m).
+  Proof.
+    clear.
+    intros. red.
+    unfold amap_lookup, amap_instantiate, amap_lookup. intros u e.
+    rewrite SUBST.FACTS.map_o.
+    consider (UVarMap.MAP.find u m); simpl; intros; try congruence.
+    inv_all. eapply H0 in H1. subst; eauto.
+  Qed.
+
+  Lemma WellFormed_bimap_instantiate
+  : forall s f min len s',
+      amap_instantiate f s = s' ->
+      (forall u e,
+         f u = Some e ->
+         forall u',
+           mentionsU u' e = true ->
+           u' < min) ->
+      WellFormed_bimap min len s ->
+      WellFormed_bimap min len s'.
+  Proof.
+    red; intros; subst.
+    red in H1. forward_reason.
+    split.
+    { red. intros.
+      rewrite SUBST.PROPS.F.find_mapsto_iff in H3.
+      unfold amap_instantiate in *.
+      rewrite SUBST.FACTS.map_o in H3.
+      red. intros.
+      consider (UVarMap.MAP.find k s); simpl in *; try congruence.
+      intros. inv_all; subst.
+      eapply SUBST.PROPS.F.not_find_in_iff.
+      rewrite SUBST.FACTS.map_o.
+      consider (UVarMap.MAP.find u s); try reflexivity.
+      intros. exfalso.
+      eapply mentionsU_instantiate in H4.
+      destruct H4.
+      { destruct H4.
+        eapply H. 2: eassumption.
+        eapply SUBST.PROPS.F.find_mapsto_iff. eassumption.
+        red. eexists.
+        eapply SUBST.PROPS.F.find_mapsto_iff. eassumption. }
+      { forward_reason.
+        specialize (H0 _ _ H4 _ H7).
+        eapply H1 in H5. omega. } }
+    split.
+    { revert H1. eapply Forall_amap_instaniate. trivial. }
+    { revert H2. eapply Forall_amap_instaniate; intros.
+      eapply mentionsU_instantiate in H3. destruct H3.
+      { destruct H3; eauto. }
+      { forward_reason.
+        eapply H0 in H3. 2: eassumption. omega. } }
+  Qed.
+
+  Definition nothing_in_range a b m : Prop :=
+    forall u, u < b -> amap_lookup (a + u) m = None.
+  Definition only_in_range min len m :=
+    Forall_amap (fun k _ => min <= k < min + len) m.
+
+  Lemma only_in_range_0_empty
+  : forall a am,
+      only_in_range a 0 am ->
+      UVarMap.MAP.Equal am amap_empty.
+  Proof.
+    clear. unfold Forall_amap. red.
+    intros.
+    specialize (H y). unfold amap_lookup in *.
+    rewrite SUBST.FACTS.empty_o.
+    destruct (UVarMap.MAP.find y am); auto.
+    exfalso. specialize (H _ eq_refl). omega.
+  Qed.
+
+  Lemma only_in_range_0_WellFormed_pre_entry
+  : forall a am,
+      only_in_range a 0 am ->
+      WellFormed_bimap a 0 am.
+  Proof.
+    clear. unfold WellFormed_bimap.
+    intros. eapply only_in_range_0_empty in H.
+    admit.
+  Qed.
+
+  (** Start pigeonhole stuff **)
+  Lemma cardinal_remove
+  : forall m x y,
+      amap_lookup x m = Some y ->
+      UVarMap.MAP.cardinal m = S (UVarMap.MAP.cardinal (UVarMap.MAP.remove x m)).
+  Proof.
+    clear. intros.
+    do 2 rewrite SUBST.PROPS.cardinal_fold.
+    assert (UVarMap.MAP.Equal m (UVarMap.MAP.add x y (UVarMap.MAP.remove x m))).
+    { red. intros.
+      rewrite SUBST.PROPS.F.add_o.
+      rewrite SUBST.PROPS.F.remove_o.
+      destruct (SUBST.PROPS.F.eq_dec x y0). subst; auto.
+      auto. }
+    etransitivity.
+    (rewrite SUBST.PROPS.fold_Equal with (eqA := @eq nat); try eassumption); eauto.
+    compute; intros; subst; auto.
+    compute; intros; subst; auto.
+    rewrite SUBST.PROPS.fold_add. reflexivity.
+    eauto.
+    compute; intros; subst; auto.
+    compute; intros; subst; auto.
+    eapply UVarMap.MAP.remove_1. reflexivity.
+  Qed.
+
+  Lemma cardinal_not_remove
+  : forall m x,
+      amap_lookup x m = None ->
+      UVarMap.MAP.cardinal m = UVarMap.MAP.cardinal (UVarMap.MAP.remove x m).
+  Proof.
+    clear. intros.
+    assert (UVarMap.MAP.Equal m (UVarMap.MAP.remove x m)).
+    { red. intros.
+      rewrite SUBST.PROPS.F.remove_o.
+      destruct (SUBST.PROPS.F.eq_dec x y). subst; auto.
+      auto. }
+    rewrite <- H0. reflexivity.
+  Qed.
+
+  Lemma subst_pull_sound
+  : forall b a m m',
+      subst_pull a b m = Some m' ->
+      nothing_in_range a b m' /\
+      UVarMap.MAP.cardinal m' = UVarMap.MAP.cardinal m - b /\
+      (forall u, u < a \/ u >= a + b -> amap_lookup u m = amap_lookup u m') /\
+      (forall u, u < b -> amap_lookup (a + u) m <> None).
+  Proof.
+    clear.
+    induction b.
+    { simpl. intros. inv_all; subst.
+      split.
+      { red. intros; exfalso; omega. }
+      split.
+      { omega. }
+      split.
+      { auto. }
+      { intros. exfalso; omega. } }
+    { simpl. unfold SUBST.raw_drop.
+      intros. forwardy.
+      eapply IHb in H. forward_reason.
+      inv_all. subst.
+      split.
+      { red. intros.
+        unfold amap_lookup. rewrite SUBST.PROPS.F.remove_o.
+        destruct (SUBST.PROPS.F.eq_dec a (a + u)); auto.
+        destruct u.
+        { exfalso; omega. }
+        { replace (a + S u) with (S a + u) by omega.
+          red in H. eapply H. omega. } }
+      split.
+      { replace (UVarMap.MAP.cardinal m - S b) with
+        ((UVarMap.MAP.cardinal m - b) - 1) by omega.
+        rewrite <- H2. clear - H0.
+        rewrite (@cardinal_remove _ _ _ H0). omega. }
+      split.
+      { intros.
+        destruct H1.
+        + rewrite H3; [ | left; eauto ].
+          unfold amap_lookup.
+          rewrite SUBST.PROPS.F.remove_neq_o; auto.
+        + rewrite H3; [ | right; omega ].
+          unfold amap_lookup.
+          rewrite SUBST.PROPS.F.remove_neq_o; auto.
+          omega. }
+      { intros.
+        destruct u.
+        { rewrite H3; [ | left; omega ].
+          replace (a + 0) with a. change_rewrite H0. congruence.
+          clear. apply plus_n_O. }
+        { replace (a + S u) with (S a + u) by omega.
+          apply H4. omega. } } }
+  Qed.
+
+  Lemma subst_pull_complete
+  : forall b a m,
+      (forall u, u < b -> amap_lookup (a + u) m <> None) ->
+      exists m',
+        subst_pull a b m = Some m'.
+  Proof.
+    clear. induction b; simpl; intros; eauto.
+    { destruct (IHb (S a) m); clear IHb.
+      { intros. replace (S a + u) with (a + S u) by omega.
+        eapply H. omega. }
+      { rewrite H0.
+        eapply subst_pull_sound in H0.
+        forward_reason. unfold SUBST.raw_drop.
+        rewrite <- H2 by (left; omega).
+        specialize (H 0).
+        replace (a + 0) with a in H by omega.
+        destruct (amap_lookup a m); eauto.
+        exfalso. eapply H; auto. omega. } }
+  Qed.
+
+  Fixpoint test_range from len m :=
+    match len with
+      | 0 => true
+      | S len =>
+        match amap_lookup from m with
+          | None => false
+          | Some _ => test_range (S from) len (UVarMap.MAP.remove from m)
+        end
+    end.
+
+  Lemma test_range_true_all
+  : forall l f m,
+      test_range f l m = true ->
+      forall u, u < l -> amap_lookup (f + u) m <> None.
+  Proof.
+    clear. induction l.
+    { intros; exfalso; omega. }
+    { simpl; intros; forward.
+      specialize (IHl _ _ H1).
+      destruct u.
+      { replace (f + 0) with f by omega. congruence. }
+      { replace (f + S u) with (S f + u) by omega.
+        cutrewrite (amap_lookup (S f + u) m =
+                    amap_lookup (S f + u) (UVarMap.MAP.remove f m)).
+        { apply IHl. omega. }
+        unfold amap_lookup.
+        rewrite SUBST.PROPS.F.remove_neq_o; auto. omega. } }
+  Qed.
+
+  Lemma cardinal_le_range
+  : forall len min m,
+      only_in_range min len m ->
+      UVarMap.MAP.cardinal m <= len.
+  Proof.
+    clear.
+    induction len.
+    { intros.
+      eapply only_in_range_0_empty in H.
+      cut (UVarMap.MAP.cardinal m = 0); try omega.
+      apply SUBST.PROPS.cardinal_1.
+      rewrite H.
+      apply UVarMap.MAP.empty_1. }
+    { intros.
+      assert (only_in_range min len (UVarMap.MAP.remove (min + len) m)).
+      { red. red in H. red. intros.
+        unfold amap_lookup in H0.
+        rewrite SUBST.PROPS.F.remove_o in H0.
+        destruct (SUBST.PROPS.F.eq_dec (min + len) u); try congruence.
+        eapply H in H0. omega. }
+      { eapply IHlen in H0.
+        consider (UVarMap.MAP.find (min + len) m); intros.
+        { erewrite cardinal_remove; eauto.
+          omega. }
+        { erewrite cardinal_not_remove; eauto. } } }
+  Qed.
+
+  Lemma subst_getInstantiation
+  : forall tus tvs ts m P,
+      WellFormed_bimap (length tus) (length ts) m ->
+      amap_substD (tus ++ ts) tvs m = Some P ->
+      amap_is_full (length ts) m = true ->
+      exists x : hlist (fun t => exprT tus tvs (typD t)) ts,
+        forall us vs,
+          let us' :=
+              hlist_map (fun t (x : exprT tus tvs (typD t)) => x us vs) x
+          in
+          P (HList.hlist_app us us') vs.
+  Proof.
+    intros.
+    assert (exists m',
+              subst_pull (length tus) (length ts) m = Some m' /\
+              UVarMap.MAP.Empty m').
+    { unfold amap_is_full in H1.
+      consider (UVarMap.MAP.cardinal m ?[ eq ] length ts); intros.
+      assert (only_in_range (length tus) (length ts) m).
+      { clear - H. red in H. red; intros.
+        tauto. }
+      clear - H1 H2.
+      destruct (@subst_pull_complete (length ts) (length tus) m).
+      { eapply test_range_true_all.
+        generalize dependent (length tus).
+        generalize dependent m.
+        induction (length ts); intros.
+        { reflexivity. }
+        { simpl.
+          consider (amap_lookup n0 m).
+          { intros.
+            eapply IHn.
+            - erewrite cardinal_remove in H1; eauto.
+            - red. intros. red. intros.
+              unfold amap_lookup in H0.
+              rewrite SUBST.PROPS.F.remove_o in H0.
+              destruct (SUBST.PROPS.F.eq_dec n0 u); try congruence.
+              eapply H2 in H0. omega. }
+          { intros. exfalso.
+            assert (only_in_range (S n0) n m).
+            { red. red; intros. red in H2.
+              consider (n0 ?[ eq ] u); intros; subst; try congruence.
+              eapply H2 in H0. omega. }
+            eapply cardinal_le_range in H0. omega. } }  }
+      rewrite H. eexists; split; eauto.
+      eapply subst_pull_sound in H.
+      assert (only_in_range (length tus) 0 x).
+      { forward_reason.
+        red. red. intros.
+        exfalso.
+        assert ((u < length tus \/ u >= length tus + length ts) \/
+                (exists u', u' < length ts /\ u = length tus + u')).
+        { consider (u ?[ lt ] length tus); try auto; intros.
+          consider (u ?[ ge ] (length tus + length ts)); try auto; intros.
+          right. exists (u - length tus). split; try omega. }
+        destruct H6.
+        { rewrite <- H3 in H5; eauto.
+          eapply H2 in H5. omega. }
+        { forward_reason. subst.
+          red in H.
+          rewrite H in H5. congruence. auto. } }
+      { eapply  only_in_range_0_empty in H0.
+        rewrite H0.
+        eapply UVarMap.MAP.empty_1. } }
+    { forward_reason.
+      eapply pull_sound in H2; eauto using SUBST.SubstOpenOk_subst.
+      { forward_reason.
+        specialize (@H4 tus ts tvs _ eq_refl eq_refl H0).
+        forward_reason.
+        exists x2. simpl. intros.
+        eapply H9.
+        assert (UVarMap.MAP.Equal x (UVarMap.MAP.empty expr)).
+        { red. red in H3. intros.
+          rewrite SUBST.FACTS.empty_o.
+          eapply SUBST.FACTS.not_find_in_iff.
+          red. intro. destruct H10. eapply H3.
+          eauto. }
+        generalize (@SUBST.raw_substD_Equal typ _ expr _ tus tvs x (UVarMap.MAP.empty _) _ H7 H10).
+        destruct (SUBST.substD_empty tus tvs).
+        intros.
+        forward_reason.
+        eapply H13; clear H13.
+        change_rewrite H12 in H11. inv_all; subst. eauto. }
+      { eapply WellFormed_bimap_WellFormed_amap; eauto. } }
+  Qed.
+
+End parameterized.
